Support for the bbT predicate

src/Trace.v
@@ -15,7 +15,7 @@
 
 
 Require Import Bool Int63 PArray.
-Require Import Misc State SMT_terms Cnf Euf Lia Syntactic Arithmetic Operators Assumptions.
+Require Import Misc State SMT_terms Cnf Euf Lia Syntactic Arithmetic Operators Assumptions BVList.
 
 Local Open Scope array_scope.
 Local Open Scope int63_scope.
@@ -231,13 +231,13 @@ Module Cnf_Checker.
     | ImmBuildProj pos cid i => S.set_clause s pos (check_ImmBuildProj t_form s cid i) 
     end.
 
-  Lemma step_checker_correct : forall rho t_form,
+  Lemma step_checker_correct : forall rho rhobv t_form,
     Form.check_form t_form ->
-    forall s, S.valid (Form.interp_state_var rho t_form) s ->
-      forall st : step, S.valid (Form.interp_state_var rho t_form)
+    forall s, S.valid (Form.interp_state_var rho rhobv t_form) s ->
+      forall st : step, S.valid (Form.interp_state_var rho rhobv t_form)
         (step_checker t_form s st).
   Proof.
-    intros rho t_form Ht s H; destruct (Form.check_form_correct rho _ Ht) as [[Ht1 Ht2] Ht3]; intros [pos res|pos cid lf|pos|pos|pos l|pos l|pos l i|pos cid|pos cid|pos cid i]; simpl; try apply S.valid_set_clause; auto.
+    intros rho rhobv t_form Ht s H; destruct (Form.check_form_correct rho rhobv _ Ht) as [[Ht1 Ht2] Ht3]; intros [pos res|pos cid lf|pos|pos|pos l|pos l|pos l i|pos cid|pos cid|pos cid i]; simpl; try apply S.valid_set_clause; auto.
     apply S.valid_set_resolve; auto.
     apply valid_check_flatten; auto; try discriminate; intros a1 a2; unfold is_true; rewrite Int63Properties.eqb_spec; intro; subst a1; auto.
     apply valid_check_True; auto.
@@ -253,12 +253,12 @@ Module Cnf_Checker.
   Definition cnf_checker t_form s t :=
     _checker_ (step_checker t_form) s t.
 
-  Lemma cnf_checker_correct : forall rho t_form,
+  Lemma cnf_checker_correct : forall rho rhobv t_form,
     Form.check_form t_form -> forall s t confl,
       cnf_checker t_form C.is_false s t confl ->
-      ~ (S.valid (Form.interp_state_var rho t_form) s).
+      ~ (S.valid (Form.interp_state_var rho rhobv t_form) s).
   Proof.
-    unfold cnf_checker; intros rho t_form Ht; apply _checker__correct.
+    unfold cnf_checker; intros rho rhobv t_form Ht; apply _checker__correct.
     intros c H; apply C.is_false_correct; auto.
     apply step_checker_correct; auto.
   Qed.
@@ -274,9 +274,9 @@ Module Cnf_Checker.
 
  Lemma checker_correct : forall t_form l c,
     checker t_form l c = true ->
-    forall rho, ~ (Lit.interp (Form.interp_state_var rho t_form) l).
+    forall rho rhobv, ~ (Lit.interp (Form.interp_state_var rho rhobv t_form) l).
  Proof.
-   unfold checker; intros t_form l (nclauses, t, confl); unfold is_true; rewrite andb_true_iff; intros [H1 H2] rho H; apply (cnf_checker_correct (rho:=rho) H1 H2); destruct (Form.check_form_correct rho _ H1) as [[Ht1 Ht2] Ht3]; apply S.valid_set_clause; auto.
+   unfold checker; intros t_form l (nclauses, t, confl); unfold is_true; rewrite andb_true_iff; intros [H1 H2] rho rhobv H; apply (cnf_checker_correct (rho:=rho) (rhobv:=rhobv) H1 H2); destruct (Form.check_form_correct rho rhobv _ H1) as [[Ht1 Ht2] Ht3]; apply S.valid_set_clause; auto.
    apply S.valid_make; auto.
    unfold C.valid; simpl; rewrite H; auto.
  Qed.
@@ -287,9 +287,9 @@ Module Cnf_Checker.
 
  Lemma checker_b_correct : forall t_var t_form l b c,
     checker_b t_form l b c = true ->
-    Lit.interp (Form.interp_state_var (PArray.get t_var) t_form) l = b.
+    Lit.interp (Form.interp_state_var (PArray.get t_var) (fun _ => BITVECTOR_LIST.bv_mk (true::nil)) t_form) l = b.
  Proof.
-   unfold checker_b; intros t_var t_form l b c; case b; case_eq (Lit.interp (Form.interp_state_var (get t_var) t_form) l); auto; intros H1 H2; elim (checker_correct H2 (rho:=get t_var)); auto; rewrite Lit.interp_neg, H1; auto.
+   unfold checker_b; intros t_var t_form l b c; case b; case_eq (Lit.interp (Form.interp_state_var (get t_var) (fun _ => BITVECTOR_LIST.bv_mk (true::nil)) t_form) l); auto; intros H1 H2; elim (checker_correct H2 (rho:=get t_var) (rhobv:=fun _ => BITVECTOR_LIST.bv_mk (true::nil))); auto; rewrite Lit.interp_neg, H1; auto.
  Qed.
 
  Definition checker_eq t_form l1 l2 l (c:certif) :=
@@ -302,12 +302,12 @@ Module Cnf_Checker.
 
  Lemma checker_eq_correct : forall t_var t_form l1 l2 l c,
    checker_eq t_form l1 l2 l c = true ->
-    Lit.interp (Form.interp_state_var (PArray.get t_var) t_form) l1 =
-    Lit.interp (Form.interp_state_var (PArray.get t_var) t_form) l2.
+    Lit.interp (Form.interp_state_var (PArray.get t_var) (fun _ => BITVECTOR_LIST.bv_mk (true::nil)) t_form) l1 =
+    Lit.interp (Form.interp_state_var (PArray.get t_var) (fun _ => BITVECTOR_LIST.bv_mk (true::nil)) t_form) l2.
  Proof.
-   unfold checker_eq; intros t_var t_form l1 l2 l c; rewrite !andb_true_iff; case_eq (t_form .[ Lit.blit l]); [intros _ _|intros _|intros _|intros _ _ _|intros _ _|intros _ _|intros _ _|intros _ _ _|intros l1' l2' Heq|intros _ _ _ _]; intros [[H1 H2] H3]; try discriminate; rewrite andb_true_iff in H2; rewrite !Int63Properties.eqb_spec in H2; destruct H2 as [H2 H4]; subst l1' l2'; case_eq (Lit.is_pos l); intro Heq'; rewrite Heq' in H1; try discriminate; clear H1; assert (H:PArray.default t_form = Form.Ftrue /\ Form.wf t_form).
-   unfold checker in H3; destruct c as (nclauses, t, confl); rewrite andb_true_iff in H3; destruct H3 as [H3 _]; destruct (Form.check_form_correct (get t_var) _ H3) as [[Ht1 Ht2] Ht3]; split; auto.
-   destruct H as [H1 H2]; case_eq (Lit.interp (Form.interp_state_var (get t_var) t_form) l1); intro Heq1; case_eq (Lit.interp (Form.interp_state_var (get t_var) t_form) l2); intro Heq2; auto; elim (checker_correct H3 (rho:=get t_var)); unfold Lit.interp; rewrite Heq'; unfold Var.interp; rewrite Form.wf_interp_form; auto; rewrite Heq; simpl; rewrite Heq1, Heq2; auto.
+   unfold checker_eq; intros t_var t_form l1 l2 l c; rewrite !andb_true_iff; case_eq (t_form .[ Lit.blit l]); [intros _ _|intros _|intros _|intros _ _ _|intros _ _|intros _ _|intros _ _|intros _ _ _|intros l1' l2' Heq|intros _ _ _ _|intros a ls Heq]; intros [[H1 H2] H3]; try discriminate; rewrite andb_true_iff in H2; rewrite !Int63Properties.eqb_spec in H2; destruct H2 as [H2 H4]; subst l1' l2'; case_eq (Lit.is_pos l); intro Heq'; rewrite Heq' in H1; try discriminate; clear H1; assert (H:PArray.default t_form = Form.Ftrue /\ Form.wf t_form).
+   unfold checker in H3; destruct c as (nclauses, t, confl); rewrite andb_true_iff in H3; destruct H3 as [H3 _]; destruct (Form.check_form_correct (get t_var) (fun _ => BITVECTOR_LIST.bv_mk (true::nil)) _ H3) as [[Ht1 Ht2] Ht3]; split; auto.
+   destruct H as [H1 H2]; case_eq (Lit.interp (Form.interp_state_var (get t_var) (fun _ => BITVECTOR_LIST.bv_mk (true::nil)) t_form) l1); intro Heq1; case_eq (Lit.interp (Form.interp_state_var (get t_var) (fun _ => BITVECTOR_LIST.bv_mk (true::nil)) t_form) l2); intro Heq2; auto; elim (checker_correct H3 (rho:=get t_var) (rhobv:=fun _ => BITVECTOR_LIST.bv_mk (true::nil))); unfold Lit.interp; rewrite Heq'; unfold Var.interp; rewrite Form.wf_interp_form; auto; rewrite Heq; simpl; rewrite Heq1, Heq2; auto.
  Qed.
 
 End Cnf_Checker.
@@ -350,7 +350,7 @@ Module Euf_Checker.
   (* Offer the possibility to discharge parts of the proof to (manual) Coq proofs.
      WARNING: this breaks extraction. *)
   | Hole (pos:int) (prem_id:list clause_id) (prem:list C.t) (concl:C.t)
-    (p:interp_conseq_uf (Form.interp_state_var (Atom.interp_form_hatom t_i t_func t_atom) t_form) prem concl)
+    (p:interp_conseq_uf (Form.interp_state_var (Atom.interp_form_hatom t_i t_func t_atom) (Atom.interp_form_hatom_bv t_i t_func t_atom) t_form) prem concl)
   .
 
   Local Open Scope list_scope.
@@ -381,13 +381,13 @@ Module Euf_Checker.
     end.
 
   Lemma step_checker_correct :
-    let rho := Form.interp_state_var (Atom.interp_form_hatom t_i t_func t_atom) t_form in
+    let rho := Form.interp_state_var (Atom.interp_form_hatom t_i t_func t_atom) (Atom.interp_form_hatom_bv t_i t_func t_atom) t_form in
       Form.check_form t_form -> Atom.check_atom t_atom ->
       Atom.wt t_i t_func t_atom ->
       forall s, S.valid rho s ->
         forall st : step, S.valid rho (step_checker s st).
   Proof.
-    intros rho H1 H2 H10 s Hs. destruct (Form.check_form_correct (Atom.interp_form_hatom t_i t_func t_atom) _ H1) as [[Ht1 Ht2] Ht3]. destruct (Atom.check_atom_correct _ H2) as [Ha1 Ha2]. intros [pos res|pos cid c|pos cid lf|pos|pos|pos l|pos l|pos l i|pos cid|pos cid|pos cid i|pos l fl|pos l fl|pos l1 l2 fl|pos cl c|pos l|pos orig res l|pos orig res|pos prem_id prem concl p]; simpl; try apply S.valid_set_clause; auto.
+    intros rho H1 H2 H10 s Hs. destruct (Form.check_form_correct (Atom.interp_form_hatom t_i t_func t_atom) (Atom.interp_form_hatom_bv t_i t_func t_atom) _ H1) as [[Ht1 Ht2] Ht3]. destruct (Atom.check_atom_correct _ H2) as [Ha1 Ha2]. intros [pos res|pos cid c|pos cid lf|pos|pos|pos l|pos l|pos l i|pos cid|pos cid|pos cid i|pos l fl|pos l fl|pos l1 l2 fl|pos cl c|pos l|pos orig res l|pos orig res|pos prem_id prem concl p]; simpl; try apply S.valid_set_clause; auto.
     - apply S.valid_set_resolve; auto.
     - apply S.valid_set_weaken; auto.
     - apply valid_check_flatten; auto; intros h1 h2 H.
@@ -415,7 +415,7 @@ Module Euf_Checker.
     _checker_ (step_checker (* t_atom t_form *)) s t.
 
   Lemma euf_checker_correct : (* forall t_i t_func t_atom t_form, *)
-    let rho := Form.interp_state_var (Atom.interp_form_hatom t_i t_func t_atom) t_form in
+    let rho := Form.interp_state_var (Atom.interp_form_hatom t_i t_func t_atom) (Atom.interp_form_hatom_bv t_i t_func t_atom) t_form in
       Form.check_form t_form -> Atom.check_atom t_atom ->
       Atom.wt t_i t_func t_atom ->
       forall s t confl,
@@ -439,17 +439,17 @@ Module Euf_Checker.
     end.
 
   Definition valid t_i t_func t_atom t_form d :=
-    let rho := Form.interp_state_var (Atom.interp_form_hatom t_i t_func t_atom) t_form in
+    let rho := Form.interp_state_var (Atom.interp_form_hatom t_i t_func t_atom) (Atom.interp_form_hatom_bv t_i t_func t_atom) t_form in
     afold_left _ _ true andb (Lit.interp rho) d.
 
   Lemma add_roots_correct : (* forall t_i t_func t_atom t_form, *)
-    let rho := Form.interp_state_var (Atom.interp_form_hatom t_i t_func t_atom) t_form in
+    let rho := Form.interp_state_var (Atom.interp_form_hatom t_i t_func t_atom) (Atom.interp_form_hatom_bv t_i t_func t_atom) t_form in
       Form.check_form t_form -> Atom.check_atom t_atom ->
       Atom.wt t_i t_func t_atom ->
       forall s d used_roots, S.valid rho s -> valid t_func t_atom t_form d ->
         S.valid rho (add_roots s d used_roots).
   Proof.
-    intros (* t_i t_func t_atom t_form *) rho H1 H2 H10 s d used_roots H3; unfold valid; intro H4; pose (H5 := (afold_left_andb_true_inv _ _ _ H4)); unfold add_roots; assert (Valuation.wf rho) by (destruct (Form.check_form_correct (Atom.interp_form_hatom t_i t_func t_atom) _ H1) as [_ H]; auto); case used_roots.
+    intros (* t_i t_func t_atom t_form *) rho H1 H2 H10 s d used_roots H3; unfold valid; intro H4; pose (H5 := (afold_left_andb_true_inv _ _ _ H4)); unfold add_roots; assert (Valuation.wf rho) by (destruct (Form.check_form_correct (Atom.interp_form_hatom t_i t_func t_atom) (Atom.interp_form_hatom_bv t_i t_func t_atom) _ H1) as [_ H]; auto); case used_roots.
     intro ur; apply (foldi_right_Ind _ _ (fun _ a => S.valid rho a)); auto; intros a i H6 Ha; apply S.valid_set_clause; auto; case_eq (ur .[ i] < length d).
     intro; unfold C.valid; simpl; rewrite H5; auto.
     intros; apply C.interp_true; auto.
@@ -467,7 +467,7 @@ Module Euf_Checker.
     checker (* t_i t_func t_atom t_form *) d used_roots c = true ->
     ~ valid t_func t_atom t_form d.
   Proof.
-    unfold checker; intros (* t_i t_func t_atom t_form *) d used_roots (nclauses, t, confl); rewrite !andb_true_iff; intros [[[H1 H2] H10] H3] H; eelim euf_checker_correct; try eassumption; apply add_roots_correct; try eassumption; apply S.valid_make; destruct (Form.check_form_correct (Atom.interp_form_hatom t_i t_func t_atom) _ H1) as [_ H4]; auto.
+    unfold checker; intros (* t_i t_func t_atom t_form *) d used_roots (nclauses, t, confl); rewrite !andb_true_iff; intros [[[H1 H2] H10] H3] H; eelim euf_checker_correct; try eassumption; apply add_roots_correct; try eassumption; apply S.valid_make; destruct (Form.check_form_correct (Atom.interp_form_hatom t_i t_func t_atom) (Atom.interp_form_hatom_bv t_i t_func t_atom) _ H1) as [_ H4]; auto.
   Qed.
 
   Definition checker_b (* t_i t_func t_atom t_form *) l (b:bool) (c:certif) :=
@@ -477,9 +477,9 @@ Module Euf_Checker.
 
   Lemma checker_b_correct : forall (* t_i t_func t_atom t_form *) l b c,
     checker_b (* t_func t_atom t_form *) l b c = true ->
-    Lit.interp (Form.interp_state_var (Atom.interp_form_hatom t_i t_func t_atom) t_form) l = b.
+    Lit.interp (Form.interp_state_var (Atom.interp_form_hatom t_i t_func t_atom) (Atom.interp_form_hatom_bv t_i t_func t_atom) t_form) l = b.
   Proof.
-   unfold checker_b; intros (* t_i t_func t_atom t_form *) l b (nclauses, t, confl); case b; intros H2; case_eq (Lit.interp (Form.interp_state_var (Atom.interp_form_hatom t_i t_func t_atom) t_form) l); auto; intros H1; elim (checker_correct H2); auto; unfold valid; apply afold_left_andb_true; intros i Hi; rewrite get_make; auto; rewrite Lit.interp_neg, H1; auto.
+   unfold checker_b; intros (* t_i t_func t_atom t_form *) l b (nclauses, t, confl); case b; intros H2; case_eq (Lit.interp (Form.interp_state_var (Atom.interp_form_hatom t_i t_func t_atom) (Atom.interp_form_hatom_bv t_i t_func t_atom) t_form) l); auto; intros H1; elim (checker_correct H2); auto; unfold valid; apply afold_left_andb_true; intros i Hi; rewrite get_make; auto; rewrite Lit.interp_neg, H1; auto.
  Qed.
 
   Definition checker_eq (* t_i t_func t_atom t_form *) l1 l2 l (c:certif) :=
@@ -493,12 +493,12 @@ Module Euf_Checker.
 
   Lemma checker_eq_correct : forall (* t_i t_func t_atom t_form *) l1 l2 l c,
     checker_eq (* t_func t_atom t_form *) l1 l2 l c = true ->
-    Lit.interp (Form.interp_state_var (Atom.interp_form_hatom t_i t_func t_atom) t_form) l1 =
-    Lit.interp (Form.interp_state_var (Atom.interp_form_hatom t_i t_func t_atom) t_form) l2.
+    Lit.interp (Form.interp_state_var (Atom.interp_form_hatom t_i t_func t_atom) (Atom.interp_form_hatom_bv t_i t_func t_atom) t_form) l1 =
+    Lit.interp (Form.interp_state_var (Atom.interp_form_hatom t_i t_func t_atom) (Atom.interp_form_hatom_bv t_i t_func t_atom) t_form) l2.
   Proof.
-   unfold checker_eq; intros (* t_i t_func t_atom t_form *) l1 l2 l (nclauses, t, confl); rewrite !andb_true_iff; case_eq (t_form .[ Lit.blit l]); [intros _ _|intros _|intros _|intros _ _ _|intros _ _|intros _ _|intros _ _|intros _ _ _|intros l1' l2' Heq|intros _ _ _ _]; intros [[H1 H2] H3]; try discriminate; rewrite andb_true_iff in H2; rewrite !Int63Properties.eqb_spec in H2; destruct H2 as [H2 H4]; subst l1' l2'; case_eq (Lit.is_pos l); intro Heq'; rewrite Heq' in H1; try discriminate; clear H1; assert (H:PArray.default t_form = Form.Ftrue /\ Form.wf t_form).
-   unfold checker in H3; rewrite !andb_true_iff in H3; destruct H3 as [[[H3 _] _] _]; destruct (Form.check_form_correct (Atom.interp_form_hatom t_i t_func t_atom) _ H3) as [[Ht1 Ht2] Ht3]; split; auto.
-   destruct H as [H1 H2]; case_eq (Lit.interp (Form.interp_state_var (Atom.interp_form_hatom t_i t_func t_atom) t_form) l1); intro Heq1; case_eq (Lit.interp (Form.interp_state_var (Atom.interp_form_hatom t_i t_func t_atom) t_form) l2); intro Heq2; auto; elim (checker_correct H3); unfold valid; apply afold_left_andb_true; intros i Hi; rewrite get_make; unfold Lit.interp; rewrite Heq'; unfold Var.interp; rewrite Form.wf_interp_form; auto; rewrite Heq; simpl; rewrite Heq1, Heq2; auto.
+   unfold checker_eq; intros (* t_i t_func t_atom t_form *) l1 l2 l (nclauses, t, confl); rewrite !andb_true_iff; case_eq (t_form .[ Lit.blit l]); [intros _ _|intros _|intros _|intros _ _ _|intros _ _|intros _ _|intros _ _|intros _ _ _|intros l1' l2' Heq|intros _ _ _ _|intros a ls Heq]; intros [[H1 H2] H3]; try discriminate; rewrite andb_true_iff in H2; rewrite !Int63Properties.eqb_spec in H2; destruct H2 as [H2 H4]; subst l1' l2'; case_eq (Lit.is_pos l); intro Heq'; rewrite Heq' in H1; try discriminate; clear H1; assert (H:PArray.default t_form = Form.Ftrue /\ Form.wf t_form).
+   unfold checker in H3; rewrite !andb_true_iff in H3; destruct H3 as [[[H3 _] _] _]; destruct (Form.check_form_correct (Atom.interp_form_hatom t_i t_func t_atom) (Atom.interp_form_hatom_bv t_i t_func t_atom) _ H3) as [[Ht1 Ht2] Ht3]; split; auto.
+   destruct H as [H1 H2]; case_eq (Lit.interp (Form.interp_state_var (Atom.interp_form_hatom t_i t_func t_atom) (Atom.interp_form_hatom_bv t_i t_func t_atom) t_form) l1); intro Heq1; case_eq (Lit.interp (Form.interp_state_var (Atom.interp_form_hatom t_i t_func t_atom) (Atom.interp_form_hatom_bv t_i t_func t_atom) t_form) l2); intro Heq2; auto; elim (checker_correct H3); unfold valid; apply afold_left_andb_true; intros i Hi; rewrite get_make; unfold Lit.interp; rewrite Heq'; unfold Var.interp; rewrite Form.wf_interp_form; auto; rewrite Heq; simpl; rewrite Heq1, Heq2; auto.
  Qed.
 
 
